theories/Parallel/ContractEquations.v
@@ -1,4 +1,4 @@
-Require Import CSL.Parallel.Contract.  
+Require Import CSL.Parallel.Contract CSL.Parallel.TranslationOnly.  
 Require Import Lists.List Bool.Bool Bool.Sumbool Setoid Coq.Arith.PeanoNat.
 From Equations Require Import Equations.
 Require Import micromega.Lia.
@@ -12,34 +12,130 @@ Set Implicit Arguments.
 
 Reserved Notation "c0 =R= c1" (at level 63).
 
+Inductive Sequential : Contract -> Prop :=
+ | SeqFailure : Sequential Failure
+ | SeqSuccess : Sequential Success
+ | SeqEvent e  : Sequential (Event e)
+ | SeqPlus c0 c1 (H0: Sequential c0) (H1 : Sequential c1) : Sequential (c0 _+_ c1)
+ | SeqSeq c0 c1 (H0: Sequential c0) (H1 : Sequential c1) : Sequential (c0 _;_ c1).
+Hint Constructors Sequential : eqDB.
+
+Definition bind {A B : Type} (a : option A) (f : A -> option B) : option B :=
+  match a with
+    | Some x => f x
+    | None => None
+  end.
+
+
+Fixpoint translate_aux (c : Contract) : option CSLC.Contract :=
+match c with
+| Failure => Some CSLC.Failure
+| Success => Some CSLC.Success
+| Event e => Some (CSLC.Event e)
+| c0 _+_ c1 => bind (translate_aux c0) (fun c0' => bind (translate_aux c1) (fun c1' => Some (CSLC.CPlus c0' c1')))
+| c0 _;_ c1 => bind (translate_aux c0) (fun c0' => bind (translate_aux c1) (fun c1' => Some (CSLC.CSeq c0' c1')))
+| c0 _*_ c1 => None
+end.
+
+Lemma translate_aux_sequential : forall (c : Contract), Sequential c -> exists c', translate_aux c = Some c'.
+Proof. 
+intros. induction H.
+- exists CSLC.Failure. reflexivity.
+- exists CSLC.Success. reflexivity.
+- exists (CSLC.Event e). reflexivity.
+- destruct IHSequential1,IHSequential2. exists (CSLC.CPlus x x0).
+  simpl. unfold bind. destruct (translate_aux c0).
+  * destruct (translate_aux c1).
+    ** inversion H1. inversion H2. reflexivity.
+    ** inversion H2.
+  * inversion H1.
+- destruct IHSequential1,IHSequential2. exists (CSLC.CSeq x x0).
+  simpl. unfold bind. destruct (translate_aux c0).
+  * destruct (translate_aux c1).
+    ** inversion H1. inversion H2. reflexivity.
+    ** inversion H2.
+  * inversion H1.
+Qed.
+
+
+Require CSL.Core.ContractEquations.
+Module CSLEQ := CSL.Core.ContractEquations.
+
+Ltac option_inversion :=
+  (repeat match goal with
+         | [ H: None = Some _ |- _ ] => discriminate
+         | [ H: Some _ = None |- _ ] => discriminate
+         | [ H: Some _ = Some _ |- _ ] => inversion H; clear H
+          end);subst.
+
+Ltac c_inversion :=
+  (repeat match goal with
+         | [ H: _ =~ Failure |- _ ] => inversion H
+         | [ H: ?s =~ _ _+_ _ |- _ ] => inversion H; clear H
+         | [ H: ?s =~ _ _;_ _ |- _ ] => inversion H; clear H
+         | [ H: ?s =~ _ _*_ _ |- _ ] => inversion H; clear H
+         | [ H: [?x] =~ Event _ |- _ ] => fail
+         | [ H: ?s =~ Event _ |- _ ] => inversion H; subst
+         | [ H: [] =~ Success |- _ ] => fail
+         | [ H: _ =~ Success |- _ ] => inversion H; clear H
+
+         end); option_inversion; auto with cDB.
+
+Ltac core_inversion := option_inversion;CSLEQ.c_inversion.
+
+Lemma translate_aux_spec : forall (c : Contract)(c' : CSLC.Contract),translate_aux c = Some c' -> (forall s, s =~ c <-> CSLC.Matches_Comp s c').
+Proof.
+split. generalize dependent c'. generalize dependent s.
+- induction c; intros;simpl in*;c_inversion.
+  all: unfold bind in H; destruct (translate_aux c1);try c_inversion;
+       destruct (translate_aux c2); c_inversion; c_inversion.
+- generalize dependent c'. generalize dependent s; induction c; intros;simpl in*.
+  * core_inversion.
+  * core_inversion.
+  * core_inversion.
+  * unfold bind in H. destruct (translate_aux c1);try c_inversion.
+    destruct (translate_aux c2);try c_inversion.
+    core_inversion; eauto with cDB.
+  * unfold bind in H. destruct (translate_aux c1);try c_inversion.
+    destruct (translate_aux c2);try c_inversion.
+    core_inversion; eauto with cDB.
+  * discriminate.
+Qed.
+
+
 Inductive c_eq : Contract -> Contract -> Prop :=
-  | c_plus_assoc c0 c1 c2 : (c0 _+_ c1) _+_ c2 =R= c0 _+_ (c1 _+_ c2)
-  | c_plus_comm c0 c1: c0 _+_ c1 =R= c1 _+_ c0
-  | c_plus_neut c: c _+_ Failure =R= c
-  | c_plus_idemp c : c _+_ c =R= c 
-  | c_seq_assoc c0 c1 c2 : (c0 _;_ c1) _;_ c2 =R= c0 _;_ (c1 _;_ c2)
-  | c_seq_neut_l c : (Success _;_ c) =R= c 
-  | c_seq_neut_r c : c _;_ Success =R= c 
-  | c_seq_failure_l c : Failure _;_ c =R= Failure    
-  | c_seq_failure_r c :  c _;_ Failure =R= Failure 
-  | c_distr_l c0 c1 c2 : c0 _;_ (c1 _+_ c2) =R= (c0 _;_ c1) _+_ (c0 _;_ c2)
-  | c_distr_r c0 c1 c2 : (c0 _+_ c1) _;_ c2 =R= (c0 _;_ c2) _+_ (c1 _;_ c2)
+| c_core p0 p1 c0 c1 (H0: translate_aux p0 = Some c0) 
+                     (H1:translate_aux p1 = Some c1)
+                     (H2: CSLEQ.c_eq c0 c1) : p0 =R= p1
 
-  | c_par_assoc c0 c1 c2 : (c0 _*_ c1) _*_ c2 =R= c0 _*_ (c1 _*_ c2)
-  | c_par_neut c : c _*_ Success =R= c 
-  | c_par_comm c0 c1: c0 _*_ c1 =R= c1 _*_ c0
-  | c_par_failure c : c _*_ Failure =R= Failure   
-  | c_par_distr_l c0 c1 c2 : c0 _*_ (c1 _+_ c2) =R= (c0 _*_ c1) _+_ (c0 _*_ c2)
+| c_plus_assoc c0 c1 c2 : (c0 _+_ c1) _+_ c2 =R= c0 _+_ (c1 _+_ c2)
+| c_plus_comm c0 c1: c0 _+_ c1 =R= c1 _+_ c0
+| c_plus_neut c: c _+_ Failure =R= c
+| c_plus_idemp c : c _+_ c =R= c 
+| c_seq_assoc c0 c1 c2 : (c0 _;_ c1) _;_ c2 =R= c0 _;_ (c1 _;_ c2)
+| c_seq_neut_l c : (Success _;_ c) =R= c 
+| c_seq_neut_r c : c _;_ Success =R= c 
+| c_seq_failure_l c : Failure _;_ c =R= Failure  
+| c_seq_failure_r c :  c _;_ Failure =R= Failure 
+| c_distr_l c0 c1 c2 : c0 _;_ (c1 _+_ c2) =R= (c0 _;_ c1) _+_ (c0 _;_ c2)
+| c_distr_r c0 c1 c2 : (c0 _+_ c1) _;_ c2 =R= (c0 _;_ c2) _+_ (c1 _;_ c2)
 
-  | c_par_event e0 e1 c0 c1 : Event e0 _;_ c0 _*_ Event e1 _;_ c1 =R= Event e0 _;_ (c0 _*_ (Event e1 _;_ c1)) _+_ Event e1 _;_ ((Event e0 _;_ c0) _*_ c1)
+| c_par_assoc c0 c1 c2 : (c0 _*_ c1) _*_ c2 =R= c0 _*_ (c1 _*_ c2)
+| c_par_neut c : c _*_ Success =R= c 
+| c_par_comm c0 c1: c0 _*_ c1 =R= c1 _*_ c0
+| c_par_failure c : c _*_ Failure =R= Failure   
+| c_par_distr_l c0 c1 c2 : c0 _*_ (c1 _+_ c2) =R= (c0 _*_ c1) _+_ (c0 _*_ c2)
 
-  | c_refl c : c =R= c
-  | c_sym c0 c1 (H: c0 =R= c1) : c1 =R= c0
-  | c_trans c0 c1 c2 (H1 : c0 =R= c1) (H2 : c1 =R= c2) : c0 =R= c2
-  | c_plus_ctx c0 c0' c1 c1' (H1 : c0 =R= c0') (H2 : c1 =R= c1') : c0 _+_ c1 =R= c0' _+_ c1'
-  | c_seq_ctx c0 c0' c1 c1' (H1 : c0 =R= c0') (H2 : c1 =R= c1') : c0 _;_ c1 =R= c0' _;_ c1'
-  | c_par_ctx c0 c0' c1 c1' (H1 : c0 =R= c0') (H2 : c1 =R= c1') : c0 _*_ c1 =R= c0' _*_ c1'
+| c_par_event e0 e1 c0 c1 : Event e0 _;_ c0 _*_ Event e1 _;_ c1 =R= Event e0 _;_ (c0 _*_ (Event e1 _;_ c1)) _+_ Event e1 _;_ ((Event e0 _;_ c0) _*_ c1)
+
+| c_refl c : c =R= c
+| c_sym c0 c1 (H: c0 =R= c1) : c1 =R= c0
+| c_trans c0 c1 c2 (H1 : c0 =R= c1) (H2 : c1 =R= c2) : c0 =R= c2
+| c_plus_ctx c0 c0' c1 c1' (H1 : c0 =R= c0') (H2 : c1 =R= c1') : c0 _+_ c1 =R= c0' _+_ c1'
+| c_seq_ctx c0 c0' c1 c1' (H1 : c0 =R= c0') (H2 : c1 =R= c1') : c0 _;_ c1 =R= c0' _;_ c1'
+| c_par_ctx c0 c0' c1 c1' (H1 : c0 =R= c0') (H2 : c1 =R= c1') : c0 _*_ c1 =R= c0' _*_ c1'
   where "c1 =R= c2" := (c_eq c1 c2).
+
 
 Hint Constructors c_eq : eqDB.
 
@@ -48,6 +144,12 @@ Add Parametric Relation : Contract c_eq
   symmetry proved by c_sym
   transitivity proved by c_trans
   as Contract_setoid.
+
+Add Parametric Morphism : Par with
+signature c_eq ==> c_eq ==> c_eq as c_eq_par_morphism.
+Proof.
+  intros. auto with eqDB.
+Qed.
 
 Add Parametric Morphism : CPlus with
 signature c_eq ==> c_eq ==> c_eq as c_eq_plus_morphism.
@@ -61,38 +163,6 @@ Proof.
   intros. auto with eqDB.
 Qed.
 
-Add Parametric Morphism : Par with
-signature c_eq ==> c_eq ==> c_eq as c_eq_par_morphism.
-Proof.
-  intros. auto with eqDB.
-Qed.
-
-
-Ltac c_inversion :=
-  (repeat match goal with
-         | [ H: _ =~ Failure |- _ ] => inversion H
-         | [ H: ?s =~ _ _+_ _ |- _ ] => inversion H; clear H
-         | [ H: ?s =~ _ _;_ _ |- _ ] => inversion H; clear H
-         | [ H: ?s =~ _ _*_ _ |- _ ] => inversion H; clear H
-         | [ H: [?x] =~ Event _ |- _ ] => fail
-         | [ H: ?s =~ Event _ |- _ ] => inversion H; subst
-         | [ H: [] =~ Success |- _ ] => fail
-         | [ H: _ =~ Success |- _ ] => inversion H; clear H
-         end);auto with cDB.
-
-
-
-
-Ltac interl_tac := 
-        (repeat match goal with
-         | [ H: _::_ = [] |- _ ] => discriminate
-         | [ H: _ /\ _ |- _ ] => destruct H
-         | [ H: _ \/ _ |- _ ] => destruct H
-         | [ H: interleave_fun _ _ [] |- _ ] => simpl in H
-         | [ H: interleave_fun _ _ (?e::?s) |- _ ] => simpl in H
-         | [ H: interleave_fun _ _ ?s |- _ ] => destruct s;simpl in H
-         | [ H: interleave _ _ _ |- _ ] => rewrite interl_iff_fun in H
-         end);subst.
 
 Lemma cons_app : forall (A: Type) (a : A)(l : list A), a::l = [a]++l.
 Proof. auto.
@@ -119,6 +189,7 @@ Qed.
 Lemma c_eq_soundness : forall (c0 c1 : Contract), c0 =R= c1 -> (forall s : Trace, s =~ c0 <-> s =~ c1).
 Proof.
 intros c0 c1 H. induction H ;intros; try solve [split;intros;c_inversion].
+  * repeat rewrite translate_aux_spec;eauto. now apply CSLEQ.c_eq_soundness.
   * split;intros;c_inversion; [ rewrite <- app_assoc | rewrite app_assoc ]; auto with cDB.
   * rewrite <- (app_nil_l s). split;intros;c_inversion.
   * rewrite <- (app_nil_r s) at 1. split;intros;c_inversion. subst.
@@ -160,6 +231,7 @@ intros c0 c1 H. induction H ;intros; try solve [split;intros;c_inversion].
                                 | rewrite IHc_eq2];auto.
 Qed.
 
+
 Lemma Matches_plus_comm : forall c0 c1 s, s =~ c0 _+_ c1 <-> s =~ c1 _+_ c0.
 Proof. auto using c_eq_soundness  with eqDB. Qed.
 
@@ -181,11 +253,24 @@ Proof. auto using c_eq_soundness  with eqDB. Qed.
 Hint Rewrite Matches_plus_neut_l 
              Matches_plus_neut_r 
              Matches_seq_neut_l
-             Matches_seq_neut_r : eqDB.
+             Matches_seq_neut_r c_par_distr_l c_par_neut c_par_failure : eqDB.
 
 Lemma c_plus_neut_l : forall c, Failure _+_ c =R= c.
 Proof. intros. rewrite c_plus_comm. auto with eqDB.
 Qed.
+
+Lemma c_par_neut_l : forall c, Success _*_ c =R= c.
+Proof. intros. rewrite c_par_comm. auto with eqDB.
+Qed.
+
+Lemma c_par_failure_l  : forall c, Failure _*_ c =R= Failure.
+Proof. intros. rewrite c_par_comm. auto with eqDB.
+Qed.
+
+Lemma c_par_distr_r : forall c0 c1 c2, (c0 _+_ c1) _*_ c2 =R= (c0 _*_ c2) _+_ (c1 _*_ c2).
+Proof. intros. rewrite c_par_comm. rewrite c_par_distr_l. auto with eqDB.
+Qed.
+
 
 Hint Rewrite c_plus_neut_l 
              c_plus_neut 
@@ -194,9 +279,898 @@ Hint Rewrite c_plus_neut_l
              c_seq_failure_l 
              c_seq_failure_r 
              c_distr_l
-             c_distr_r : eqDB.
+             c_distr_r c_par_neut_l c_par_failure_l c_par_distr_r c_par_event : eqDB.
 
 Ltac auto_rwd_eqDB := autorewrite with eqDB;auto with eqDB.
+
+
+
+
+Definition alphabet := [Notify;Transfer].
+
+Lemma in_alphabet : forall e, In e alphabet.
+Proof.
+destruct e ; repeat (try apply in_eq ; try apply in_cons).
+Qed.
+
+Hint Resolve in_alphabet : eqDB.
+Opaque alphabet.
+
+Fixpoint Σ (l : list Contract) : Contract :=
+match l with
+| [] => Failure
+| c ::l => c _+_ (Σ l)
+end.
+
+(*Maybe not needed*)
+Lemma Σ_app : forall (l1 l2 : list Contract), 
+Σ (l1 ++ l2) =R= (Σ l1) _+_ (Σ l2).
+Proof.
+induction l1;intros;simpl;auto_rwd_eqDB.
+rewrite IHl1. now rewrite c_plus_assoc.
+Qed.
+
+(*Not used in this file, maybe used in decision procedure*)
+Lemma in_Σ : forall (l : list Contract)(s : Trace), s =~ Σ l <-> 
+(exists c, In c l /\ s =~ c).
+Proof. 
+induction l;intros;simpl.
+- split;intros. c_inversion. destruct_ctx. contradiction.
+- split;intros. c_inversion. exists a. split;auto.
+  rewrite IHl in H1. destruct_ctx. exists x. split;auto.
+  destruct_ctx. inversion H. subst. auto with cDB.
+  apply MPlusR. rewrite IHl. exists x. split;auto.
+Qed.
+
+Lemma in_Σ_idemp : forall l c, In c l -> c _+_ Σ l =R= Σ l.
+Proof.
+induction l;intros;simpl; auto_rwd_eqDB.
+simpl in H;contradiction.
+simpl in H. destruct H. subst. all: rewrite <- c_plus_assoc.
+auto_rwd_eqDB. rewrite (c_plus_comm c). rewrite c_plus_assoc. 
+apply c_plus_ctx;auto_rwd_eqDB.
+Qed. 
+
+Lemma incl_Σ_idemp : forall (l1 l2 : list Contract), incl l1 l2 -> Σ l2 =R= Σ (l1++l2).
+Proof. 
+induction l1;intros;simpl;auto_rwd_eqDB.
+apply incl_cons_inv in H as [H0 H1].
+rewrite <- IHl1;auto. now rewrite in_Σ_idemp;auto.
+Qed.
+
+Lemma Σ_app_comm : forall (l1 l2 : list Contract), Σ (l1++l2) =R= Σ (l2++l1).
+Proof.
+induction l1;intros;simpl. now rewrite app_nil_r.
+repeat rewrite Σ_app. rewrite <- c_plus_assoc.
+rewrite c_plus_comm. apply c_plus_ctx;auto_rwd_eqDB.
+Qed.
+
+Lemma incl_Σ_c_eq : forall (l1 l2 : list Contract), incl l1 l2 -> incl l2 l1-> Σ l1 =R= Σ l2.
+Proof.
+intros. rewrite (incl_Σ_idemp H). 
+rewrite (incl_Σ_idemp H0). apply Σ_app_comm.
+Qed.
+
+
+Equations plus_norm (c : Contract) : (Contract) by  wf (con_size c) :=
+plus_norm  c := if stuck_dec c then Failure
+               else if nu c then Success _+_ Σ (map (fun e => (Event e) _;_ (plus_norm (e \ c))) alphabet)
+                            else             Σ (map (fun e => (Event e) _;_ (plus_norm (e \ c))) alphabet).
+
+Next Obligation. auto using not_stuck_derives. Defined.
+Next Obligation. auto using not_stuck_derives. Defined.
+Global Transparent plus_norm.
+
+
+Lemma plus_norm_cons : forall (e:EventType)(s:Trace)(c:Contract),
+(forall (e : EventType) (s : Trace), s =~ e \ c <-> s =~ plus_norm (e \ c)) ->
+e :: s =~ c <-> e :: s =~ Σ (map (fun e0 : EventType => Event e0 _;_ plus_norm (e0 \ c)) alphabet).
+Proof.
+intros. repeat rewrite derive_spec_comp.
+assert (HA: forall (l : list Contract)(e : EventType), e \ (Σ l) = Σ (map (fun c => e \ c) l)).
+{ intros. induction l. - reflexivity. - simpl. f_equal. assumption. } rewrite HA. rewrite in_Σ.
+rewrite map_map. rewrite H. split;intros.
+- exists (Success _;_ (plus_norm (e \ c))). split.
+  * rewrite in_map_iff. exists e. split;auto with eqDB. 
+    simpl. destruct (EventType_eq_dec e e);[ reflexivity | contradiction ].
+  * rewrite <- (app_nil_l s). constructor; auto with cDB.
+- destruct H0 as [c0 [P0 P1]]. rewrite in_map_iff in P0. destruct P0 as [x [P3 P4]]. subst.
+  simpl in P1. destruct (EventType_eq_dec x e).
+  * inversion P1. inversion H3. subst. simpl. assumption.
+  * inversion P1. inversion H3.
+Qed.
+
+
+Lemma plus_norm_nil : forall (c : Contract), ~([] =~ Σ (map (fun e0 : EventType => Event e0 _;_ plus_norm (e0 \ c)) alphabet)).
+Proof.
+intros. intro H. apply in_Σ in H as [c0 [P0 P1]]. apply in_map_iff in P0 as [e [P P3]]. 
+subst. inversion P1. apply app_eq_nil in H0 as [H0 H00]. subst. inversion H1.
+Qed.
+ 
+Theorem plus_norm_spec : forall (c : Contract)(s : Trace), s =~ c <-> s =~ plus_norm c.
+Proof.
+intros. funelim (plus_norm c). destruct (stuck_dec c).
+- apply Stuck_failure. assumption.
+- destruct (nu c) eqn:Heqn.
+  * destruct s.
+    ** split;intros;auto with cDB. auto using Matches_Comp_nil_nu. 
+    ** assert (HA: forall (c : Contract), e::s =~ Success _+_ c <-> e::s =~ c).
+       { split; intros. inversion H0. inversion H3. assumption. auto with cDB. } rewrite HA.
+       apply plus_norm_cons. auto.
+  * destruct s.
+    ** split;intros.
+      *** rewrite Matches_Comp_iff_matchesb in H0. simpl in H0. 
+          rewrite Heqn in H0. discriminate.
+      *** apply plus_norm_nil in H0 as [].
+    ** apply plus_norm_cons. auto.
+Qed.
+
+Lemma Stuck_eq_Failure : forall c, Stuck c -> c =R= Failure.
+Proof.
+intros. induction H;auto with eqDB.
+- rewrite IHStuck1. rewrite IHStuck2. auto_rwd_eqDB.
+- rewrite IHStuck. auto_rwd_eqDB.
+- rewrite IHStuck. rewrite c_par_comm. auto_rwd_eqDB.
+- rewrite IHStuck. auto_rwd_eqDB.
+Qed.
+
+Ltac stuck_tac := 
+   match goal with
+    | [ |- context[if stuck_dec ?c then _ else _ ]] => destruct (stuck_dec c)
+        end.
+
+Lemma plus_norm_Failure : plus_norm Failure =R= Failure.
+Proof.
+simp plus_norm. stuck_tac;auto_rwd_eqDB. inversion n.
+Qed. 
+
+Lemma Σ_Seq_Failure : forall es, Σ (map (fun e : EventType => Event e _;_ plus_norm Failure) es) =R= Failure.
+Proof.
+induction es. simpl. reflexivity.
+simpl. rewrite IHes. auto_rwd_eqDB.
+Qed.
+
+Lemma plus_norm_Success : plus_norm Success =R= Success.
+Proof.
+simp plus_norm. stuck_tac. symmetry. auto using Stuck_eq_Failure.
+simpl. rewrite Σ_Seq_Failure. auto_rwd_eqDB.
+Qed. 
+
+Hint Rewrite plus_norm_Failure plus_norm_Success : eqDB.
+
+Lemma map_ext_in_R :
+  forall (A : Type)(f g:A->Contract) l, (forall a, In a l -> f a =R= g a) -> Σ (map f l) =R= Σ (map g l).
+Proof.
+induction l;intros;simpl;auto with eqDB.
+apply c_plus_ctx. apply H. apply in_eq. apply IHl.
+intros. apply H. simpl. now right.
+Qed.
+
+(*
+Lemma ext_in_map_R :
+  forall (A : Type)(f g:A->Contract) l, Σ (map f l) =R= Σ (map g l) -> forall a, In a l -> f a =R= g a.
+Proof.
+induction l;intros. simpl in H0. contradiction.
+simpl in H0. destruct H0.
+- subst. simpl in H. apply IHl. apply map_ext_in_R.
+*)
+
+Inductive Atom : Contract -> Prop :=
+| AFailure : Atom Failure
+| ASuccess : Atom Success.
+
+Inductive NormalForm : Contract -> Prop :=
+| NFF: NormalForm Failure
+| NFS: NormalForm Success
+| NFList es l (H1: forall a, In a l -> NormalForm a) : NormalForm (Σ (map (fun x => Event (fst x) _;_ snd x) (combine es l)))
+| NFListS es l  (H1: forall a, In a l -> NormalForm a) : NormalForm (Success _+_ Σ (map (fun x => Event (fst x) _;_ snd x) (combine es l))).
+
+Lemma Sequential_Σ : forall l, Forall Sequential l -> Sequential (Σ l).
+Proof.
+induction l;intros.
+- simpl. constructor.
+- simpl. rewrite Forall_forall in H. constructor.
+  apply H. apply in_eq. apply IHl. rewrite <- Forall_forall in H.
+  inversion H. auto.
+Qed.
+
+
+Lemma NormalForm_i_Sequential : forall c, NormalForm c -> Sequential c.
+Proof.
+intros. induction H;auto with eqDB.
+- apply Sequential_Σ. rewrite Forall_forall in *. intros.
+  rewrite in_map_iff in H0. destruct_ctx. subst. constructor.
+  constructor. destruct x0. apply in_combine_r in H2. auto.
+- constructor;auto with eqDB. apply Sequential_Σ. rewrite Forall_forall in *. intros.
+  rewrite in_map_iff in H0. destruct_ctx. subst. constructor.
+  constructor. destruct x0. apply in_combine_r in H2. auto.
+Qed.
+
+Lemma NormalForm_trans : forall c, NormalForm c -> exists c', translate_aux c = Some c'.
+Proof.
+intros. apply translate_aux_sequential. auto using NormalForm_i_Sequential.
+Qed.
+
+
+Lemma Σ_extend : forall l c, c _+_ Σ l = Σ (c :: l ).
+Proof.
+induction l;intros. auto. simpl. auto.
+Qed.
+
+Lemma decompose_map : 
+forall es c, map (fun e => Event e _;_ plus_norm (e \ c)) es = map (fun x => (Event (fst x) _;_ snd x)) (combine es (map (fun e => plus_norm (e \ c) ) es)).
+Proof.
+induction es;intros.
+- simpl. auto.
+- simpl. rewrite IHes. auto.
+Qed. 
+
+Lemma plus_norm_NormalForm : forall c, NormalForm (plus_norm c).
+Proof.
+intros. funelim (plus_norm c). stuck_tac.
+- constructor.
+- destruct (nu c).
+  * rewrite decompose_map. erewrite map_ext. eapply NFListS.
+    intros. rewrite in_map_iff in H0. destruct_ctx.
+    subst. auto. intros. destruct a. simpl. auto.
+  * rewrite decompose_map. erewrite map_ext. eapply NFList.
+    intros. rewrite in_map_iff in H0. destruct_ctx.
+    subst. auto. intros. destruct a. simpl. auto.
+Qed.
+
+Lemma plus_norm_trans : forall c, exists c', translate_aux (plus_norm c) = Some c'.
+Proof.
+intros. eauto using plus_norm_NormalForm, NormalForm_trans.
+Qed.
+(*
+Lemma plus_norm_core : forall c0 c1 c0' c1', tra c0 = Some c0' -> translate c1 = Some c1'
+-> (forall s, s=~ c0 <-> s =~ c1 ) -> c0' =R= c1'.*)
+(*
+Lemma NormalFormEvent : forall l e , 
+NormalForm (Σ (map (fun e0 => Event e0 _;_ plus_norm (if EventType_eq_dec e e0 then Success else Failure)) l)).
+Proof.
+intros.
+induction l;intros.
+- simpl. constructor. constructor.
+- simpl. eq_event_destruct;subst.
+  * rewrite Σ_extend. constructor. rewr con*)
+
+(*
+Lemma Σ_Seq_Event : forall alphabet0 e, (forall e', In e' alphabet0) ->
+Σ
+  (map (fun e0 : EventType => Event e0 _;_ plus_norm (if EventType_eq_dec e e0 then Success else Failure))
+     alphabet0) =R= Event e.
+Proof. intros.
+eapply c_core;simpl;eauto. destruct e. simpl.
+induction alphabet0;intros.
+- simpl in H. contradiction.
+- simpl. rewrite IHalphabet0.
+intros.*)
+(*
+Fixpoint translate_aux_core c :=
+match c with
+| CSLC.Failure => CSLC.Failure
+| CSLC.Event e => CSLEQ.Σ (map (fun e1 => CSLC.CSeq (CSLC.Event e1) (CSLC.derive e)(if EventType_eq_dec e e1 then CSLC.Success else CSLC.Failure)) alphabet0)).
+
+Lemma translate_aux_Event : forall alphabet0 e x, 
+translate_aux (Σ (map (fun e0 : EventType => Event e0 _;_ plus_norm (if EventType_eq_dec e e0 then Success else Failure)) alphabet0)) =
+Some x -> CSLEQ.c_eq x
+(CSLEQ.Σ (map (fun e1 => CSLC.CSeq (CSLC.Event e1) (if EventType_eq_dec e e1 then CSLC.Success else CSLC.Failure)) alphabet0)).
+Proof.
+induction alphabet0;intros. 
+- simpl in*. inversion H;subst. constructor.
+- simpl. eq_event_destruct;subst.
+  * rewrite IHalphabet0. simpl. auto.
+intros.
+    Some x
+
+Lemma trans_plus_norm_Event : forall e x, translate_aux (plus_norm (Event e)) = Some x -> CSLEQ.c_eq (CSLC.Event e) x.
+Proof. 
+intros. simp plus_norm in H. simpl in H.*)
+
+Lemma derive_Success : forall e, e \ Success = Failure.
+Proof.
+intros. destruct e;auto.
+Qed.
+(*
+Lemma Σ_event : forall l e c, (forall c', In c' (c::l) -> c =R= Failure \/ c =R= Event e) -> Σ (c::l) =R= Event e.
+Proof.
+induction l;intros.
+simpl. auto_rwd_eqDB. specialize 
+now right.
+simpl. left. specialize IHl with e. simpl in H.
+specialize H with a.
+-
+simpl.
+
+*)
+
+Lemma Σ_event : forall l e,
+Σ (map (fun a => Event e _;_ (if EventType_eq_dec e a then Success else Failure)) l) =R= 
+Event e _;_  Σ (map (fun a => (if EventType_eq_dec e a then Success else Failure)) l).
+Proof.
+induction l;intros.
+- simpl. auto_rwd_eqDB.
+- simpl. rewrite IHl. auto_rwd_eqDB.
+Qed.
+
+Lemma or_imp : forall (A B C : Prop), (A \/ B -> C) -> (A -> C) /\ (B -> C). 
+Proof.
+intros. split;auto.
+Qed.
+(*
+Lemma Σ_Success : forall l, (exists c, In c l /\ c =R= Success) -> (forall c, In c l -> c =R= Success \/ c =R= Failure) -> Σ l =R= Success.
+Proof.
+induction l;intros.
+- destruct_ctx. simpl in H. contradiction.
+- destruct_ctx. simpl in *. destruct H.
+  subst.
+  * rewrite H1. rewrite IHl.
+  * specialize H0 with a. apply or_imp in H0. destruct H0.
+    destruct H0;auto. rewrite H0. auto_rwd_eqDB.
+    rewrite H0. auto_rwd_eqDB.
+  *
+
+destruct H;subst.
+    ** rewrite H1. auto_rwd_eqDB.
+    ** specialize H0 with a. apply or_imp in H0. destruct H0.
+       destruct H0;auto. rewrite H0.
+  * destruct H;s ubst.
+    ** rewrite H1. 
+  rewrite IHl. auto_rwd_eqDB.  subst. simpl.*)
+
+
+Lemma Σ_alphabet_or : forall alphabet0 e ,
+ Σ (map (fun a : CSLC.EventType => if EventType_eq_dec e a then Success else Failure) alphabet0) =R= Success /\ In e alphabet0 \/
+ Σ (map (fun a : CSLC.EventType => if EventType_eq_dec e a then Success else Failure) alphabet0) =R= Failure /\ ~(In e alphabet0).
+Proof.
+induction alphabet0;intros.
+- simpl. now right.
+- simpl. eq_event_destruct.
+  * subst. edestruct IHalphabet0.
+    ** destruct H. left. split.
+       rewrite H. auto_rwd_eqDB. now left.
+    ** destruct H. rewrite H.
+       auto_rwd_eqDB.
+  * edestruct IHalphabet0.
+    ** destruct H. rewrite H. auto_rwd_eqDB.
+    ** destruct H. rewrite H. auto_rwd_eqDB.
+       right. split;auto with eqDB. intro H2. destruct H2.
+       symmetry in H1. contradiction. contradiction.
+Qed.
+
+Lemma Σ_alphabet : forall e, Σ (map (fun a => if EventType_eq_dec e a then Success else Failure) alphabet) =R= Success.
+Proof.
+intros. destruct (Σ_alphabet_or alphabet e).
+- destruct H. auto.
+- destruct H. pose proof (in_alphabet e). contradiction.
+Qed.
+
+Lemma Σ_decompose_fun : forall (A: Type) l (P P' : A -> Contract),
+Σ (map (fun a : A => P a _+_ P' a) l) =R= Σ (map (fun a : A => P a) l) _+_  Σ (map (fun a : A => P' a) l).
+Proof.
+induction l;intros.
+- simpl. auto_rwd_eqDB.
+- simpl. rewrite c_plus_assoc. rewrite c_plus_assoc. apply c_plus_ctx;auto with eqDB.
+  rewrite (c_plus_comm (Σ _)).
+  rewrite c_plus_assoc. apply c_plus_ctx;auto with eqDB. rewrite IHl.
+  auto_rwd_eqDB.
+Qed.
+
+Lemma Σ_decompose_Seq : forall l (P: EventType -> Contract) c,
+Σ (map (fun a  => P a _;_ c) l) =R= Σ (map (fun a  => P a) l) _;_ c.
+Proof.
+induction l;intros.
+- simpl. auto_rwd_eqDB.
+- simpl. auto_rwd_eqDB.
+Qed.
+
+Lemma Σ_decompose_Seq_l : forall l (P: EventType -> Contract) c,
+Σ (map (fun a  => c _;_ P a) l) =R= c _;_ Σ (map (fun a  => P a) l).
+Proof.
+induction l;intros.
+- simpl. auto_rwd_eqDB.
+- simpl. auto_rwd_eqDB.
+Qed.
+
+
+Lemma Σ_par_distr_aux : forall l1 c (P' : EventType -> Contract),
+c _*_ Σ (map (fun a0 : EventType => P' a0) l1) =R=
+Σ (map (fun a' : EventType => c _*_ P' a') l1).
+Proof.
+induction l1;intros.
+- simpl. auto_rwd_eqDB.
+- simpl. rewrite <- IHl1. auto_rwd_eqDB.
+Qed.
+
+Lemma Σ_par_distr : forall l0 l1 (P P' : EventType -> Contract),
+Σ (map (fun a  => P a) l0) _*_ Σ (map (fun a => P' a) l1) =R=
+Σ (map (fun aa  => P (fst aa) _*_ P' (snd aa)) (list_prod l0 l1)).
+Proof. 
+induction l0;intros.
+- simpl. auto_rwd_eqDB.
+- simpl.  auto_rwd_eqDB.
+  rewrite map_app. rewrite Σ_app. apply c_plus_ctx.
+  * rewrite map_map. simpl. apply Σ_par_distr_aux.
+  * auto_rwd_eqDB.
+Qed. 
+
+
+Lemma Σ_par_distr_aux_r : forall l1 c (P' : EventType -> Contract),
+Σ (map (fun a0 : EventType => P' a0) l1) _*_ c =R=
+Σ (map (fun a' : EventType => P' a' _*_ c) l1).
+Proof.
+induction l1;intros.
+- simpl. auto_rwd_eqDB.
+- simpl. rewrite <- IHl1. auto_rwd_eqDB.
+Qed.
+(*
+Lemma Σ_par_distr_r : forall l0 l1 (P P' : EventType -> Contract),
+Σ (map (fun a  => P a) l0) _*_ Σ (map (fun a => P' a) l1) =R=
+Σ (map (fun aa  => P (fst aa) _*_ P' (snd aa)) (list_prod l0 l1)).
+Proof. 
+induction l0;intros.
+- simpl. auto_rwd_eqDB.
+- simpl.  auto_rwd_eqDB.
+  rewrite map_app. rewrite Σ_app. apply c_plus_ctx.
+  * rewrite map_map. simpl. apply Σ_par_distr_aux.
+  * auto_rwd_eqDB.
+Qed. *)
+
+Definition o c := if nu c then Success else Failure.
+
+Lemma o_plus : forall c0 c1, o (c0 _+_ c1) =R= o c0 _+_ o c1.
+Proof.
+unfold o. intros. simpl. destruct (nu c0);destruct (nu c1);simpl;auto_rwd_eqDB.
+Qed.
+
+Lemma o_seq : forall c0 c1, o (c0 _;_ c1) =R= o c0 _;_ o c1.
+Proof.
+unfold o. intros. simpl. destruct (nu c0);destruct (nu c1);simpl;auto_rwd_eqDB.
+Qed.
+
+Lemma o_par : forall c0 c1, o (c0 _*_ c1) =R= o c0 _*_ o c1.
+Proof.
+unfold o. intros. simpl. destruct (nu c0);destruct (nu c1);simpl;auto_rwd_eqDB.
+Qed.
+
+
+Lemma o_true : forall c, nu c = true -> o c = Success.
+Proof.
+intros. unfold o. destruct (nu c);auto. discriminate.
+Qed. 
+
+Lemma o_false : forall c, nu c = false -> o c = Failure.
+Proof.
+intros. unfold o. destruct (nu c);auto. discriminate.
+Qed. 
+
+Lemma o_destruct : forall c, o c = Success \/ o c = Failure.
+Proof.
+intros. unfold o. destruct (nu c);auto || auto.
+Qed.
+
+Hint Rewrite o_plus o_seq o_par : eqDB.
+
+Hint Rewrite o_true o_false : oDB.
+
+Ltac eq_m_left := repeat rewrite c_plus_assoc; apply c_plus_ctx;
+                  auto_rwd_eqDB.
+
+Ltac eq_m_right := repeat rewrite <- c_plus_assoc; apply c_plus_ctx;
+                  auto_rwd_eqDB.
+(*
+Lemma derive_eq : forall e c,
+o c _+_ Event e _;_ e \ c =R= c  \/
+e \ c =R= Failure.
+Proof.
+induction c;intros;simpl.
+- left. auto_rwd_eqDB. 
+- left. auto_rwd_eqDB.
+- eq_event_destruct;auto_rwd_eqDB. subst. now left.
+- destruct IHc1; destruct IHc2.
+  * rewrite <- H at 3. rewrite <- H0 at 3. left.
+    auto_rwd_eqDB. rewrite (c_plus_assoc _ (_ _;_ _)).
+    rewrite (c_plus_comm (_ _;_ _) (o c2 _+_ _)).
+    eq_m_left.
+  * rewrite H0. auto_rwd_eqDB. left. rewrite c_plus_assoc. 
+    rewrite (c_plus_comm _ (_ _;_ _)). rewrite <- c_plus_assoc.
+    rewrite H. (o _)). 
+
+    
+    destruct (nu c1). simpl. 
+    ** destruct (nu c2).
+      *** auto_rwd_eqDB. rewrite c_plus_assoc. rewrite (c_plus_comm _ (Success _+_ _)).
+          repeat rewrite <- (c_plus_assoc). rewrite c_plus_idemp.
+          repeat rewrite c_plus_assoc.  
+          apply c_plus_ctx. reflexivity. auto_rwd_eqDB.
+      *** auto_rwd_eqDB.
+    ** simpl. destruct (nu c2).
+      *** auto_rwd_eqDB. rewrite c_plus_comm.
+          repeat rewrite c_plus_assoc. apply c_plus_ctx.
+          reflexivity. auto_rwd_eqDB.
+      *** auto_rwd_eqDB.
+  *
+ _ Success) .
+          rewrite c_plus_comm. specialize IHc1 with e. destruct IHc1.
+  * left. setoid_rewrite <- H at 3. destruct_ctx. setoid_rewrite H0 at 1. 
+  setoid_rewrite H at 1.*)
+(*
+Lemma test : forall alphabet0 c1 c2,
+Σ (map (fun a : EventType => Event a _;_ (a \ c1 _*_ c2)) alphabet0) _+_ Σ (map (fun a : EventType => Event a _;_ (c1 _*_ a \ c2)) alphabet0) =R=
+o c1 _*_ (Σ (map (fun a : EventType => Event a _;_ a \ c2) alphabet0) _+_
+o c2 _*_ Σ (map (fun a : EventType => Event a _;_ a \ c1) alphabet0) _+_
+Σ (map (fun a : EventType => Event a _;_ a \ c1) alphabet0)) _*_ Σ (map (fun a : EventType => Event a _;_ a \ c2) alphabet0) .
+Proof.
+induction alphabet0;intros.
+- simpl. auto_rwd_eqDB.
+- simpl. rewrite (c_plus_comm (Event a _;_ (c1 _*_ a \ c2))).
+  repeat rewrite <- (c_plus_assoc _ (Σ _)) .
+  rewrite (c_plus_assoc (_ _;_ _)). rewrite IHalphabet0.
+  destruct (o_destruct c1); rewrite H in *.
+  * destruct (o_destruct c2); rewrite H0 in *.
+    ** repeat rewrite (c_par_neut_l).
+       auto_rwd_eqDB.
+       rewrite (c_par_comm (_ _+_ _)).
+       auto_rwd_eqDB. 
+       rewrite (c_plus_comm ((Σ _) _*_ (Σ _))).
+       rewrite <- (c_plus_comm (_ _;_ (c1 _*_ a \ c2))).
+Check c_par_event.
+       rewrite <- c_plus_assoc.
+
+    autorewrite with eqDB in *.
+    **
+   in H. rewrite IHalphabet0.*)
+
+Lemma fold_Failure : forall l, Σ (map (fun _ : EventType => Failure) l) =R= Failure.
+Proof.
+induction l;intros. simpl. reflexivity.
+simpl. rewrite IHl. autorewrite with eqDB. reflexivity.
+Qed.
+
+Lemma Σ_list_prod_aux : forall l1 a c1 c2,
+Event a _;_ (a \ c1 _*_ Σ (map (fun a0 : EventType => Event a0 _;_ a0 \ c2) l1)) =R=
+Σ (map (fun a0 : EventType * EventType => Event (fst a0) _;_ (fst a0 \ c1 _*_ Event (snd a0) _;_ snd a0 \ c2)) (map (fun y : EventType => (a, y)) l1)).
+Proof.
+induction l1;intros;simpl.
+- auto_rwd_eqDB.
+- rewrite map_map. simpl. 
+  auto_rwd_eqDB. apply c_plus_ctx;auto with eqDB.
+  rewrite IHl1. rewrite map_map. simpl. reflexivity.
+Qed.
+
+
+Lemma Σ_list_prod : forall l0 l1 c1 c2,
+Σ (map (fun a => Event a _;_ (a \ c1 _*_ Σ (map (fun a0 : EventType => Event a0 _;_ a0 \ c2) l1))) l0) =R=
+Σ (map (fun a : EventType * EventType => Event (fst a) _;_ (fst a \ c1 _*_ Event (snd a) _;_ snd a \ c2)) (list_prod l0 l1)).
+Proof.
+induction l0;intros;simpl.
+- reflexivity.
+- rewrite map_app. rewrite Σ_app. rewrite IHl0. apply c_plus_ctx;auto with eqDB.
+  apply Σ_list_prod_aux.
+Qed.
+
+
+
+
+Lemma ΣΣ_prod : forall l0 l1 (P : EventType * EventType -> Contract), 
+Σ (map (fun a  => P a) (list_prod l0 l1))  =R=
+Σ (map (fun a0 => Σ (map (fun a1 => P (a0,a1)) l1)) l0).
+Proof.
+induction l0;intros.
+- simpl. reflexivity.
+- simpl. rewrite map_app. rewrite Σ_app.
+  eq_m_left. rewrite map_map. reflexivity.
+Qed. 
+(*
+
+Lemma Σ_plus_decompose
+Σ (map (fun a0 : EventType => P (a, a0) _+_ Σ (map (fun a1 : EventType => P (a1, a0)) l0)) l1)
+*)
+Lemma ΣΣ_prod_swap : forall l0 l1 (P : EventType * EventType -> Contract), 
+Σ (map (fun a0 => Σ (map (fun a1 => P (a0,a1)) l1)) l0)=R=
+Σ (map (fun a0 => Σ (map (fun a1 => P (a1,a0)) l0)) l1).
+Proof.
+induction l0;intros.
+- simpl. induction l1;intros;simpl;auto with eqDB. rewrite IHl1.
+  auto with eqDB.
+- simpl. rewrite Σ_decompose_fun. eq_m_left.
+Qed.
+
+
+
+Ltac rwd_in_map f := rewrite map_ext_in_R ; try instantiate (1:=f);intros; auto_rwd_eqDB.
+
+Lemma derive_unfold : forall c, o c _+_ Σ (map (fun a : EventType => Event a _;_ a \ c) alphabet) =R= c.
+Proof.
+induction c;intros;simpl in *;auto_rwd_eqDB.
+- rwd_in_map (fun (_ : EventType) => Failure).
+  induction alphabet. simpl. auto_rwd_eqDB.
+  simpl. rewrite IHl. auto_rwd_eqDB. 
+- auto_rwd_eqDB. rwd_in_map (fun a => Event e _;_ (if EventType_eq_dec e a then Success else Failure)).
+  * rewrite Σ_event. rewrite Σ_alphabet. auto_rwd_eqDB.
+  * intros. eq_event_destruct;subst. reflexivity.
+    auto_rwd_eqDB.
+- rwd_in_map (fun a => Event a _;_ a \ c1  _+_  Event a _;_ a \ c2);
+  intros; auto_rwd_eqDB.  rewrite Σ_decompose_fun. 
+  rewrite <- c_plus_assoc. rewrite (c_plus_comm (o _)).
+rewrite (c_plus_assoc (o _)).
+  rewrite IHc1. rewrite (c_plus_comm _ c1).
+  rewrite c_plus_assoc. rewrite IHc2. auto_rwd_eqDB.
+- destruct (nu c1) eqn:Heqn.
+  * rwd_in_map (fun a => Event a _;_ a \ c1 _;_ c2  _+_  Event a _;_ a \ c2);
+    intros; auto_rwd_eqDB.  rewrite Σ_decompose_fun.
+    rewrite Σ_decompose_Seq. rewrite <- IHc1 at 2.
+    rewrite <- IHc2 at 2. rewrite <- IHc2 at 3. auto_rwd_eqDB. eq_m_left.
+    apply o_true in Heqn. rewrite Heqn.
+    auto_rwd_eqDB. rewrite (c_plus_comm (Σ _ _;_ Σ _ )).
+    eq_m_right. 
+  * apply o_false in Heqn. rewrite Heqn in*. autorewrite with eqDB in *.
+    rwd_in_map (fun a => Event a _;_ a \ c1 _;_ c2);
+    intros; auto_rwd_eqDB. rewrite Σ_decompose_Seq. 
+    rewrite IHc1. reflexivity.
+- auto_rwd_eqDB.
+  rewrite (map_ext_in_R _ (fun a : EventType =>  ((Event a _;_ (a \ c1 _*_ o c2) _+_ Event a _;_ ( a \ c1 _*_Σ (map (fun a : EventType => Event a _;_ a \ c2) alphabet))) 
+_+_ (Event a _;_ (o c1 _*_ a \ c2) _+_ Event a _;_ (Σ (map (fun a : EventType => Event a _;_ a \ c1) alphabet) _*_ a \ c2 )))));
+
+  try solve [intros; rewrite <- c_distr_l; rewrite <- c_par_distr_l;  rewrite IHc2;
+  rewrite <- c_distr_l; rewrite <- c_distr_l;
+  rewrite <- c_par_distr_r; rewrite IHc1; reflexivity].
+  rewrite <- IHc1 at 2.
+  rewrite <- IHc2 at 2.
+  auto_rwd_eqDB. repeat rewrite (c_par_comm (_ _+_ _)). auto_rwd_eqDB.
+  rewrite c_plus_assoc. eq_m_left. 
+repeat rewrite Σ_decompose_fun.
+repeat rewrite <- c_plus_assoc. 
+remember (Σ (map (fun a : EventType => Event a _;_ (a \ c1 _*_ Σ (map (fun a0 : EventType => Event a0 _;_ a0 \ c2) alphabet))) alphabet)) as a.
+remember (Σ (map (fun a0 : EventType => Event a0 _;_ (Σ (map (fun a1 : EventType => Event a1 _;_ a1 \ c1) alphabet) _*_ a0 \ c2)) alphabet)) as b.
+repeat rewrite c_plus_assoc. rewrite (c_plus_comm a).
+repeat rewrite <- c_plus_assoc.
+rewrite (c_plus_assoc _ b).
+apply c_plus_ctx.
+  * rewrite c_plus_comm. apply c_plus_ctx.
+    ** destruct (o_destruct c1).
+      *** rewrite H. auto_rwd_eqDB. apply map_ext_in_R;
+          intros; auto_rwd_eqDB.
+      *** rewrite H. auto_rwd_eqDB. 
+          rewrite (map_ext_in_R _ (fun _ : EventType => Failure)).
+          apply fold_Failure. intros. auto_rwd_eqDB.
+    ** destruct (o_destruct c2).
+      *** rewrite H. auto_rwd_eqDB. apply map_ext_in_R.
+          intros. auto_rwd_eqDB.
+      *** rewrite H. auto_rwd_eqDB. 
+          rewrite (map_ext_in_R _ (fun _ : EventType => Failure)).
+          apply fold_Failure. intros. auto_rwd_eqDB.
+  * subst. rewrite Σ_par_distr.
+rewrite (map_ext_in_R _ ((fun a : EventType * EventType =>  Event (fst a) _;_ (fst a \ c1 _*_ Event (snd a) _;_ snd a \ c2) _+_ 
+Event (snd a) _;_ (Event (fst a) _;_ fst a \ c1 _*_ snd a \ c2))));
+    intros; auto_rwd_eqDB. rewrite Σ_decompose_fun.
+ rewrite c_plus_comm. repeat rewrite ΣΣ_prod;simpl. apply c_plus_ctx.
+    ** apply map_ext_in_R. intros. rewrite Σ_decompose_Seq_l.
+       rewrite <- Σ_par_distr_aux. reflexivity.
+    ** pose proof (ΣΣ_prod_swap alphabet alphabet
+(fun p => Event (snd p) _;_ (Event (fst p) _;_ (fst p) \ c1 _*_ (snd p) \ c2))).
+       simpl in H. rewrite H. apply map_ext_in_R.
+       intros. rewrite Σ_decompose_Seq_l. apply c_seq_ctx;auto with eqDB.
+       rewrite Σ_par_distr_aux_r. reflexivity.
+Qed.
+
+(*
+Lemma derive_unfold : forall c, (if nu c then Success else Failure) _+_ Σ (map (fun a : EventType => Event a _;_ a \ c) alphabet) =R= c.
+Proof.
+induction c;intros;simpl in *.
+- rewrite (map_ext_in_R _ (fun _ => Failure)).
+  induction alphabet. simpl. auto_rwd_eqDB.
+  simpl. rewrite <- c_plus_assoc. rewrite (c_plus_comm Success).
+  rewrite c_plus_assoc.
+  rewrite IHl. auto_rwd_eqDB.
+  intros. destruct a;simpl; auto_rwd_eqDB.
+- rewrite (map_ext_in_R _ (fun _ => Failure)).
+  induction alphabet. simpl. auto_rwd_eqDB.
+  simpl. rewrite <- c_plus_assoc.
+  rewrite c_plus_idemp. apply IHl. 
+  intros. destruct a;simpl; auto_rwd_eqDB.
+- auto_rwd_eqDB. 
+ rewrite (map_ext_in_R _ (fun a => Event e _;_ (if EventType_eq_dec e a then Success else Failure))).
+  * rewrite Σ_event. rewrite Σ_alphabet. auto_rwd_eqDB.
+  * intros. eq_event_destruct;subst. reflexivity.
+    auto_rwd_eqDB.
+- rewrite (map_ext_in_R _ (fun a => Event a _;_ a \ c1  _+_  Event a _;_ a \ c2));
+  intros; auto_rwd_eqDB.  rewrite Σ_decompose_fun.
+  destruct (nu c1);simpl.
+  * destruct (nu c2);simpl.
+    ** rewrite <- (c_plus_idemp Success).
+       rewrite c_plus_assoc. rewrite <- (c_plus_assoc _ (Σ _)).
+       rewrite IHc1. rewrite (c_plus_comm c1). rewrite <- c_plus_assoc.
+       rewrite IHc2. auto_rwd_eqDB.
+    ** autorewrite with eqDB in IHc2. rewrite IHc2.
+       rewrite <- c_plus_assoc. rewrite IHc1. reflexivity.
+  * destruct (nu c2);simpl.
+    ** autorewrite with eqDB in IHc1. rewrite IHc1.
+       rewrite (c_plus_comm c1). rewrite <- c_plus_assoc.  rewrite IHc2.
+       auto_rwd_eqDB. 
+    ** autorewrite with eqDB in *. rewrite IHc1. rewrite IHc2. reflexivity.
+- destruct (nu c1 && nu c2) eqn:Heqn.
+  * apply andb_prop in Heqn. destruct Heqn. rewrite H in*.
+    rewrite H0 in *.
+    rewrite (map_ext_in_R _ (fun a => Event a _;_ a \ c1 _;_ c2  _+_  Event a _;_ a \ c2));
+    intros; auto_rwd_eqDB.  rewrite Σ_decompose_fun.
+    rewrite Σ_decompose_Seq. rewrite <- IHc1.
+    rewrite <- IHc2. rewrite (c_distr_l (Success _+_ _)).
+    repeat rewrite (c_distr_r). auto_rwd_eqDB.
+    rewrite (c_plus_assoc Success). apply c_plus_ctx;auto with eqDB.
+    rewrite c_plus_assoc. apply c_plus_ctx;auto with eqDB.
+  * rewrite andb_false_iff in Heqn. destruct Heqn.
+    ** rewrite H in*. rewrite (map_ext_in_R _ (fun a => Event a _;_ a \ c1 _;_ c2));
+       intros; auto_rwd_eqDB. rewrite Σ_decompose_Seq. 
+          autorewrite with eqDB in IHc1. rewrite IHc1. reflexivity.
+    ** rewrite H in*. destruct (nu c1) eqn:Heqn.
+      *** rewrite (map_ext_in_R _ (fun a => Event a _;_ a \ c1 _;_ c2  _+_  Event a _;_ a \ c2));
+          intros; auto_rwd_eqDB.  rewrite Σ_decompose_fun.
+          rewrite Σ_decompose_Seq. autorewrite with eqDB in IHc2.
+          rewrite <- IHc1. auto_rwd_eqDB.
+          rewrite <- IHc2. auto_rwd_eqDB.
+      *** rewrite (map_ext_in_R _ (fun a => Event a _;_ a \ c1 _;_ c2));
+          intros; auto_rwd_eqDB. rewrite Σ_decompose_Seq.
+          autorewrite with eqDB in IHc1. rewrite IHc1. reflexivity.
+- rewrite <- IHc1 at 2.
+  rewrite <- IHc2 at 2.
+  auto_rwd_eqDB. repeat rewrite (c_par_comm (_ _+_ _)). auto_rwd_eqDB.
+  rewrite c_plus_assoc. apply c_plus_ctx.
+  * destruct (nu c1); destruct (nu c2);simpl;auto_rwd_eqDB.
+  *
+  rewrite 
+ destruct (nu c1 && nu c2) eqn:Heqn.
+  * apply andb_prop in Heqn. destruct Heqn.
+ rewrite H in*. 
+    rewrite H0 in IHc2.
+ Check c_par_event.
+    rewrite (map_ext_in_R _ (fun a => Event a _;_ (a \ c1 _*_ c2)  _+_  Event a _;_ (c1 _*_ a \ c2)));
+          intros; auto_rwd_eqDB.
+ Check c_par_event. 
+rewrite Σ_decompose_fun.
+ Check c_par_event.
+    rewrite <- IHc1.
+    rewrite <-  rewrite <- (c_par_comm c2). auto_rwd_eqDB.
+    rewrite <- IHc2. repeat rewrite (c_par_comm (_ _+_ _)).
+    auto_rwd_eqDB. rewrite Σ_par_distr. 
+ Check c_par_event.*)
+
+Lemma plus_norm_c_eq : forall c, plus_norm c =R= c.
+Proof.
+intros. funelim (plus_norm c).
+stuck_tac.
+- symmetry. auto using Stuck_eq_Failure.
+- destruct (nu c) eqn:Heqn.
+  * rewrite map_ext_in_R. 2: { intros. rewrite H at 1;auto. eapply c_refl. }
+ 
+  * reflexivity.
+induction c;intros.
+4: { simp plus_norm. stuck_tac.
+  * inversion s.
+    apply Stuck_eq_Failure in H2. apply Stuck_eq_Failure in H3.
+    rewrite H2. rewrite H3. auto_rwd_eqDB.
+  * simpl. destruct (nu c1 || nu c2) eqn:Heqn.
+    **
+- auto_rwd_eqDB. 
+- auto_rwd_eqDB. 
+
+Lemma plus_norm_c_eq : forall c, plus_norm c =R= c.
+Proof.
+induction c;intros.
+4: { simp plus_norm. stuck_tac.
+  * inversion s.
+    apply Stuck_eq_Failure in H2. apply Stuck_eq_Failure in H3.
+    rewrite H2. rewrite H3. auto_rwd_eqDB.
+  * simpl. destruct (nu c1 || nu c2) eqn:Heqn.
+    **
+- auto_rwd_eqDB. 
+- auto_rwd_eqDB. 
+
+- destruct (plus_norm_trans (Event e)).
+  eapply c_core;simpl;  eauto. symmetry. auto using trans_plus_norm_Event.
+
+
+  apply trans_plus_norm_Event in H.
+  pose proof (translate_aux_spec H). eapply NormalForm_trans. simp plus_norm. stuck_tac. symmetry. auto using Stuck_eq_Failure.
+  simpl. pose proof in_alphabet. induction alphabet. 
+  specialize H with Transfer. simpl in H. contradiction.
+   simpl. rewrite IHl. eq_event_destruct;subst.
+   auto_rwd_eqDB. auto_rwd_eqDB. rewrite e0 in e1. discriminate.
+  * auto_rwd_eqDB.
+
+ apply Stuck_eq_Failure.  simp plus_norm. auto with eqDB.
+
+Section axiomatization.
+
+  Hypothesis sum_rule : forall c, exists c', NormalForm c' /\ c =R= c'.
+
+  Lemma c_eq_completeness : forall (c0 c1 : Contract),(forall s : Trace, s =~ c0 <-> s =~ c1) ->  c0 =R= c1.
+  Proof.
+  intros. destruct (sum_rule c0). destruct (sum_rule c1). destruct_ctx.
+  pose proof c_eq_soundness H3. setoid_rewrite H4 in H. 
+  pose proof c_eq_soundness H2. setoid_rewrite H5 in H.
+  rewrite H3. rewrite H2.
+  apply NormalForm_trans in H0. apply NormalForm_trans in H1. destruct_ctx. 
+  eapply c_core. eauto. eauto. apply CSLEQ.c_eq_completeness.
+  setoid_rewrite <- translate_aux_spec. eapply H. all: eauto.
+  Qed.
+
+End axiomatization.
+ 
+
+
+
+
+
+
+Lemma plus_norm_sequential : forall (c : Contract), Sequential (plus_norm c).
+Proof. 
+intros. funelim (plus_norm c).
+destruct (stuck_dec c).
+- constructor.
+- destruct (nu c).
+  * constructor. constructor. induction alphabet.
+    ** simpl. constructor.
+    ** simpl. repeat constructor. auto. assumption.
+  * induction alphabet.
+    ** simpl. constructor.
+    ** simpl. repeat constructor. auto. assumption.
+Defined.
+
+
+
+(*
+Lemma stuck_c_eq_Failure : forall c c', translate_aux c = Some c' -> Stuck c -> CSLEQ.c_eq CSLC.Failure c'.
+Proof. Admitted.*)
+
+Ltac core_tac := eapply c_core;simpl;eauto with eqDB.
+
+Lemma stuck_c_eq_Failure : forall c, Stuck c -> Failure =R= c.
+Proof.
+intros. induction H; try solve [core_tac].
+- rewrite <- IHStuck1. rewrite <- IHStuck2. core_tac.
+- rewrite <- IHStuck.
+
+Lemma plus_norm_eq : forall p, plus_norm p =R= p.
+Proof. 
+intros. funelim (plus_norm p). destruct (stuck_dec c).
+- induction s.
+  * eapply c_core;simpl;eauto with eqDB.
+  * destruct (translate_aux c) eqn:Heqn.
+  * apply stuck_c_eq_Failure in Heqn as H';auto. eapply c_core;simpl;eauto.
+  *
+    simpl. eauto. eapply Heqn. eauto.
+    simpl. inversion s.
+
+
+
+Theorem c_eq_complete : forall c0 c1, (forall s, s =~ c0 <-> s=~c1) -> c0 =R= c1.
+Proof.
+intros. rewrite <- plus_norm_eq. rewrite <- (plus_norm_eq c1).
+destruct (correct_translation c0). destruct (correct_translation c1).
+destruct_ctx. unfold translate in *.
+ eapply c_core;eauto. apply CSLEQ.c_eq_completeness. 
+ setoid_rewrite <- H3. setoid_rewrite <- H2. auto.
+Qed.
+
+
+
+
+
+
+
+
+
+
+
+
+
+Inductive NormalForm : list Contract -> Prop :=
+| NF_nil : NormalForm []
+| NF_cons e c l (H: NormalForm l) : NormalForm ((Event e _;_ c):: l).
+
+
 
 Equations interleavings  (s0 s1: Trace) : (list Trace) by  wf ((length s0) + (length s1)) :=
 interleavings [] s1 := [s1];
@@ -326,7 +1300,7 @@ Proof.
 intros. unfold incl. intros. rewrite <- Matches_iff_member in *. auto.
 Qed.
 
-Lemma comp_equiv_destruct : forall (c0 c1: Contract),(forall s : Trace, s =~ c0 <-> s =~ c1) <->
+Lemma comc_equiv_destruct : forall (c0 c1: Contract),(forall s : Trace, s =~ c0 <-> s =~ c1) <->
 (forall s : Trace, s =~ c0 -> s =~ c1) /\ (forall s : Trace, s =~ c1 -> s =~ c0).
 Proof.
  split ; intros.
@@ -338,64 +1312,10 @@ Qed.
 Theorem Matches_eq_i_incl_and : forall (c0 c1 : Contract), (forall (s : Trace), s =~ c0 <-> s =~ c1) -> 
 incl (L c0) (L c1) /\ incl (L c1) (L c0) .
 Proof.
-intros. apply comp_equiv_destruct in H. destruct H. split; auto using Matches_incl. 
+intros. apply comc_equiv_destruct in H. destruct H. split; auto using Matches_incl. 
 Qed.
 
 
-Fixpoint Σ (l : list Contract) : Contract :=
-match l with
-| [] => Failure
-| c ::l => c _+_ (Σ l)
-end.
-
-(*Maybe not needed*)
-Lemma Σ_app : forall (l1 l2 : list Contract), 
-Σ (l1 ++ l2) =R= (Σ l1) _+_ (Σ l2).
-Proof.
-induction l1;intros;simpl;auto_rwd_eqDB.
-rewrite IHl1. now rewrite c_plus_assoc.
-Qed.
-
-(*Not used in this file, maybe used in decision procedure*)
-Lemma in_Σ : forall (l : list Contract)(s : Trace), s =~ Σ l <-> 
-(exists c, In c l /\ s =~ c).
-Proof. 
-induction l;intros;simpl.
-- split;intros. c_inversion. destruct_ctx. contradiction.
-- split;intros. c_inversion. exists a. split;auto.
-  rewrite IHl in H1. destruct_ctx. exists x. split;auto.
-  destruct_ctx. inversion H. subst. auto with cDB.
-  apply MPlusR. rewrite IHl. exists x. split;auto.
-Qed.
-
-Lemma in_Σ_idemp : forall l c, In c l -> c _+_ Σ l =R= Σ l.
-Proof.
-induction l;intros;simpl; auto_rwd_eqDB.
-simpl in H;contradiction.
-simpl in H. destruct H. subst. all: rewrite <- c_plus_assoc.
-auto_rwd_eqDB. rewrite (c_plus_comm c). rewrite c_plus_assoc. 
-apply c_plus_ctx;auto_rwd_eqDB.
-Qed. 
-
-Lemma incl_Σ_idemp : forall (l1 l2 : list Contract), incl l1 l2 -> Σ l2 =R= Σ (l1++l2).
-Proof. 
-induction l1;intros;simpl;auto_rwd_eqDB.
-apply incl_cons_inv in H as [H0 H1].
-rewrite <- IHl1;auto. now rewrite in_Σ_idemp;auto.
-Qed.
-
-Lemma Σ_app_comm : forall (l1 l2 : list Contract), Σ (l1++l2) =R= Σ (l2++l1).
-Proof.
-induction l1;intros;simpl. now rewrite app_nil_r.
-repeat rewrite Σ_app. rewrite <- c_plus_assoc.
-rewrite c_plus_comm. apply c_plus_ctx;auto_rwd_eqDB.
-Qed.
-
-Lemma incl_Σ_c_eq : forall (l1 l2 : list Contract), incl l1 l2 -> incl l2 l1-> Σ l1 =R= Σ l2.
-Proof.
-intros. rewrite (incl_Σ_idemp H). 
-rewrite (incl_Σ_idemp H0). apply Σ_app_comm.
-Qed.
 
 
 Fixpoint Π (s : Trace) :=
@@ -440,13 +1360,7 @@ apply c_plus_ctx; auto using Π_distr_aux2 with eqDB.
 Qed.*)
 
 (*Mention in report*)
-Lemma map_ext_in_R :
-  forall (A : Type)(f g:A->Contract) l, (forall a, In a l -> f a =R= g a) -> Σ (map f l) =R= Σ (map g l).
-Proof.
-induction l;intros;simpl;auto with eqDB.
-apply c_plus_ctx. apply H. apply in_eq. apply IHl.
-intros. apply H. simpl. now right.
-Qed.
+
 
 Lemma exchange : forall p q r s, 
  (p _*_ q) _;_ (r _*_ s) _+_ (p _;_ r) _*_ (q _;_ s) =R= (p _;_ r) _*_ (q _;_ s).
