theories/Parallel/Translation.v
@@ -1,0 +1,411 @@
+Require Import Lists.List.
+Require Import Bool.Bool.
+Require Import Bool.Sumbool.
+Require Import Program.
+From Equations Require Import Equations.
+Require Import micromega.Lia.
+Require Import Arith.
+Import ListNotations.
+
+Require Import CSL.Parallel.Contract.
+
+Set Implicit Arguments.
+
+
+
+Inductive Stuck : Contract -> Prop :=
+ | STFailure : Stuck Failure
+ | STPLus c0 c1 (H0 : Stuck c0) (H1 : Stuck c1) : Stuck (c0 _+_ c1)
+ | STSeq c0 c1 (H0 : Stuck c0) : Stuck (c0 _;_ c1)
+ | STParL c0 c1 (H0 : Stuck c0) : Stuck (c0 _*_ c1)
+ | STParR c0 c1 (H1 : Stuck c1) : Stuck (c0 _*_ c1).
+Hint Constructors Stuck : tDB.
+
+Inductive NotStuck : Contract -> Prop :=
+ | NSTSuccess : NotStuck Success
+ | NSEvent e : NotStuck (Event e)
+ | NSTPlusL c0 c1 (H0 : NotStuck c0) : NotStuck (c0 _+_ c1)
+ | NSTPlusR c0 c1 (H1 : NotStuck c1) : NotStuck (c0 _+_ c1)
+ | NSTSeq c0 c1 (H0 : NotStuck c0) : NotStuck (c0 _;_ c1)
+ | NSTPar c0 c1 (H0 : NotStuck c0)(H1 : NotStuck c1) : NotStuck (c0 _*_ c1).
+
+Hint Constructors NotStuck : tDB.
+
+Fixpoint stuck (c : Contract) :=
+match c with
+| Failure => true
+| c0 _+_ c1 => stuck c0 && stuck c1
+| c0 _;_ _ => stuck c0
+| c0 _*_ c1 => stuck c0 || stuck c1
+| _ => false
+end.
+
+
+
+Lemma stuck_false : forall (c : Contract), stuck c = false -> NotStuck c.
+Proof.
+induction c; intros;simpl in*;auto with tDB bool; try discriminate.
+apply andb_false_elim in H as [H | H]; auto with tDB.
+apply orb_false_iff in H as [H1 H2]; auto with tDB.
+Defined.
+
+Lemma stuck_true : forall (c : Contract), stuck c = true -> (Stuck c).
+Proof.
+induction c; intros; simpl in *; auto with tDB; try discriminate. 
+apply orb_prop in H as [H | H]; auto with tDB.
+Defined.
+
+
+Definition stuck_dec (c : Contract) : {Stuck c}+{NotStuck c}.
+Proof. destruct (stuck c) eqn:Heqn; auto using stuck_true || auto using stuck_false.
+Defined.
+
+Lemma NotStuck_negation : forall (c : Contract), NotStuck c -> ~(Stuck c).
+Proof.
+intros. induction H ; intro H2; inversion H2.
+all : inversion H2; contradiction.
+Qed.
+
+Fixpoint con_size (c:Contract):nat :=
+match c with
+| Failure => 0
+| Success => 1
+| Event _ => 2
+| c0 _+_ c1 => max (con_size c0) (con_size c1) 
+| c0 _;_ c1 => if stuck_dec c0 then 0 else (con_size c0) + (con_size c1)
+| c0 _*_ c1 => if  sumbool_or _ _ _ _ (stuck_dec c0) (stuck_dec c1) then 0 else (con_size c0) + (con_size c1)
+end.
+
+Ltac stuck_tac :=
+  (repeat match goal with
+         | [ H : _ /\ _ |- _ ] => destruct H
+         | [ |- context[if ?a then _ else _] ] => destruct a
+         | [ H: Stuck ?c0, H1: NotStuck ?c0  |- _ ] => apply NotStuck_negation in H1; contradiction
+  end);auto with tDB.
+
+
+
+Lemma stuck_0 : forall (c : Contract), Stuck c -> con_size c = 0.
+Proof.
+intros. induction H;auto;simpl; try solve [ lia | stuck_tac].
+Defined.
+
+Lemma stuck_not_nullary : forall (c : Contract), Stuck c -> nu c = false.
+Proof.
+intros. induction H; simpl ;subst ;auto with bool.
+all : rewrite IHStuck. all: auto with bool.
+rewrite andb_comm. auto with bool.
+Defined.
+
+Lemma Stuck_derive : forall (c : Contract)(e : EventType), Stuck c -> Stuck (e \ c).
+Proof.
+intros. induction H; simpl in *.
+- constructor.
+- constructor; auto.
+- apply stuck_not_nullary in H. rewrite H. auto with tDB.
+- auto with tDB.
+- auto with tDB.
+Qed.
+
+
+
+Lemma Stuck_derive_0 : forall (c : Contract)(e:EventType), Stuck c -> con_size (e \ c) = 0.
+Proof.
+intros. apply stuck_0. apply Stuck_derive. assumption.
+Qed.
+
+Ltac NotStuck_con H := apply NotStuck_negation in H; contradiction.
+
+Lemma NotStuck_0lt : forall (c : Contract), NotStuck c -> 0 < con_size c.
+Proof.
+intros. induction H; simpl ; try lia.
+- stuck_tac. lia.
+- stuck_tac. destruct o; stuck_tac. lia.
+Defined.
+(*
+Lemma not_stuck_derives : forall (c : Contract), NotStuck c -> (forall (e : EventType), con_size (e \ c ) < con_size c).
+Proof.
+intros. generalize dependent e. induction H;intros;simpl.
+- lia.
+- stuck_tac.
+- apply NotStuck_0lt in H. apply Max.max_case_strong. intros.
+  unfold lt. lia.
+*)
+
+Lemma lt_le_l : forall n0 n1 n2 n3, n0 <= n2 -> n1 < n3 -> n0 + n1 < n2 + n3.
+Proof.
+intros. lia.
+Qed.
+
+Lemma lt_le_r : forall n0 n1 n2 n3, n0 < n2 -> n1 <= n3 -> n0 + n1 < n2 + n3.
+Proof.
+intros. lia.
+Qed.
+
+Lemma S_plus : forall n, S n = 1 + n.
+Proof.
+lia.
+Qed.
+
+Lemma not_stuck_derives : forall (c : Contract), NotStuck c -> (forall (e : EventType), con_size (e \ c) < con_size c).
+Proof.
+intros. induction c.
+- simpl. lia.
+- inversion H.
+- simpl. destruct (EventType_eq_dec e0 e) ; simpl ; lia.
+- simpl. inversion H.
+  * destruct (stuck_dec c2).
+    ** apply stuck_0 in s as s2. rewrite (Stuck_derive_0 _ s). rewrite Max.max_comm. simpl. 
+       apply Max.max_case_strong.
+      *** intros. auto.
+      *** intros. rewrite s2 in H3. pose proof (NotStuck_0lt H1). lia.
+    ** apply IHc1 in H1. apply IHc2 in n. lia.
+  * destruct (stuck_dec c1).
+    ** apply stuck_0 in s as s2. rewrite (Stuck_derive_0 _ s). simpl. 
+       apply Max.max_case_strong.
+      *** intros. rewrite s2 in H3. pose proof (NotStuck_0lt H0). lia.
+      *** intros. auto.
+    ** apply IHc1 in n. apply IHc2 in H0. lia.
+- inversion H. subst. simpl. destruct (nu c1) eqn:Heqn.
+  * destruct (stuck_dec c1). apply NotStuck_negation in H1. contradiction.
+    simpl. destruct (stuck_dec (e \ c1)).
+    ** simpl. destruct (stuck_dec c2).
+      *** rewrite Stuck_derive_0. pose proof (NotStuck_0lt H1). lia. assumption.
+      *** rewrite <- (plus_O_n (con_size (e \ c2))). apply IHc2 in n0. lia.
+    ** apply IHc1 in H1. destruct (stuck_dec c2).
+
+      *** rewrite (Stuck_derive_0 _ s). rewrite Max.max_comm.  simpl. apply plus_lt_compat_r.  assumption. 
+      *** apply IHc1 in n. apply IHc2 in n1. lia.
+  * destruct (stuck_dec c1).
+    ** apply NotStuck_negation in H1. contradiction.
+    ** simpl. destruct (stuck_dec (e \ c1)).
+      *** pose proof (NotStuck_0lt H1). lia.
+      *** apply Plus.plus_lt_compat_r. auto.
+- inversion H. subst. simpl. destruct (sumbool_or (Stuck (e \ c1)) (NotStuck (e \ c1))
+                                      (Stuck c2) (NotStuck c2) (stuck_dec (e \ c1))
+      (                                 stuck_dec c2)) as [[o | o] | o].
+  * destruct (sumbool_or (Stuck c1) (NotStuck c1) 
+      (Stuck (e \ c2)) (NotStuck (e \ c2)) 
+      (stuck_dec c1) (stuck_dec (e \ c2))) as [[o0 | o0] | o0].
+    ** NotStuck_con H2.
+    ** simpl. destruct (sumbool_or (Stuck c1) (NotStuck c1) (Stuck c2)
+    (NotStuck c2) (stuck_dec c1) (stuck_dec c2)) as [[o1 | o1] | o1].
+      *** NotStuck_con H2.
+      *** NotStuck_con H3.
+      *** pose proof (NotStuck_0lt H2). lia.
+    ** destruct (sumbool_or (Stuck c1) (NotStuck c1) (Stuck c2)
+    (NotStuck c2) (stuck_dec c1) (stuck_dec c2)) as [[o1 | o1] | o1].
+      *** NotStuck_con H2. 
+      *** NotStuck_con H3. 
+      *** simpl. apply plus_lt_compat_l. auto. 
+  * NotStuck_con H3. 
+  * destruct o. destruct (sumbool_or (Stuck c1) (NotStuck c1) 
+      (Stuck (e \ c2)) (NotStuck (e \ c2)) 
+      (stuck_dec c1) (stuck_dec (e \ c2))) as [[o0 | o0] | o0].
+    ** NotStuck_con H2. 
+    ** destruct (sumbool_or (Stuck c1) (NotStuck c1) (Stuck c2)
+    (NotStuck c2) (stuck_dec c1) (stuck_dec c2)) as [[o | o] | o].
+      *** NotStuck_con H2.
+      *** NotStuck_con H3.
+      *** rewrite Max.max_comm. simpl. apply plus_lt_compat_r. auto.
+    ** destruct (sumbool_or (Stuck c1) (NotStuck c1) (Stuck c2)
+    (NotStuck c2) (stuck_dec c1) (stuck_dec c2)) as [[o | o] | o].
+      *** NotStuck_con H2.
+      *** NotStuck_con H3.
+      *** apply Max.max_case_strong. 
+        **** intros. apply plus_lt_compat_r. auto.
+        **** intros. apply plus_lt_compat_l. auto.
+Qed.
+
+(*
+Fixpoint plus_fold (l : list Contract) : Contract :=
+match l with
+| [] => Failure
+| c ::l => c _+_ (plus_fold l)
+end.
+
+Lemma in_plus_fold : forall (s : Trace)(l : list Contract), s ==~ plus_fold l <-> 
+(exists c, In c l /\ s ==~ c).
+Proof.
+intros. split.
+- induction l.
+  * intros. simpl in H. inversion H.
+  * intros. simpl in H. inversion H. 
+    ** exists a. split. apply in_eq. assumption.
+    ** apply IHl in H1 as [c' [P1 P2]]. exists c'. split ; auto using  in_cons.
+- intros. destruct H as [ c' [P1 P2]]. induction l.
+  * destruct P1.
+  * apply in_inv in P1 as [P1 | P1].
+    ** simpl. rewrite P1. auto.
+    ** simpl. auto.
+Qed.*)
+
+
+Lemma Stuck_failure : forall (c : Contract), Stuck c -> (forall s, s ==~ c <-> s ==~ Failure).
+Proof.
+intros. split. 2: { intros. inversion H0. }
+generalize dependent s.  induction c; intros.
+- inversion H.
+- assumption. 
+- inversion H.
+- inversion H. inversion H0; auto.
+- inversion H. inversion H0. apply IHc1 in H7. inversion H7. assumption.
+- inversion H0. inversion H.
+  * eapply IHc1 in H8. inversion H8. eauto.
+  * eapply IHc2 in H8. inversion H8. eauto.
+Qed.
+
+
+
+Equations plus_norm (c : Contract) : (Contract) by  wf (con_size c) :=
+plus_norm  c := if stuck_dec c then Failure
+               else if nu c then Success _+_ plus_fold (map (fun e => (Event e) _;_ (plus_norm (c / e))) alphabet)
+                            else             plus_fold (map (fun e => (Event e) _;_ (plus_norm (c / e))) alphabet).
+
+Next Obligation. auto using not_stuck_derives. Defined.
+Next Obligation. auto using not_stuck_derives. Defined.
+Global Transparent plus_norm.
+Eval compute in plus_norm (Transfer _._ Notify _._ Success _+_ Success).
+
+
+(*
+Lemma empty_nu : forall (c : Contract), [] ==~ c <-> nu c = true.
+Proof.
+intros. split. 
+- induction c; intros.
+  * reflexivity.
+  * inversion H.
+  * inversion H.
+  * inversion H. { simpl. rewrite IHc1; try assumption. reflexivity. }
+                { simpl. rewrite IHc2; try assumption. rewrite orb_comm.  reflexivity. }
+  * simpl. inversion H. apply app_eq_nil in H1 as [H11 H12]. subst. rewrite IHc1. rewrite IHc2. reflexivity.
+  all: assumption.
+  * inversion H. inversion H5; subst;simpl.
+    ** rewrite IHc1. rewrite IHc2. reflexivity. all:auto.
+    ** rewrite IHc1. rewrite IHc2. reflexivity. all:auto.
+- intros. induction c.
+  * constructor.
+  * discriminate H.
+  * discriminate H.
+  * simpl in H. apply orb_prop in H as [H | H]; auto.
+  * simpl in H. rewrite <- (app_nil_l []). apply andb_prop in H as [H1 H2]; auto.
+  * simpl in H. apply andb_prop in H as [H1 H2]. apply MPar with [] []; auto. 
+Qed.*)
+
+
+Lemma plus_norm_cons : forall (e:EventType)(s:Trace)(c:Contract),
+(forall (e : EventType) (s : Trace), s ==~ c / e <-> s ==~ plus_norm (c / e)) ->
+e :: s ==~ c <-> e :: s ==~ plus_fold (map (fun e0 : EventType => Event e0 _;_ plus_norm (c / e0)) alphabet).
+Proof.
+intros. repeat rewrite derive_spec_comp.
+assert (HA: forall (l : list Contract)(e : EventType), (plus_fold l) / e = plus_fold (map (fun c => c / e) l)).
+{ intros. induction l. - reflexivity. - simpl. f_equal. assumption. } rewrite HA. rewrite in_plus_fold.
+rewrite map_map. rewrite H. split;intros.
+- exists (Success _;_ (plus_norm (c / e))). split.
+  * rewrite in_map_iff. exists e. split. 
+      ** simpl. destruct (eq_event_dec e e);[ reflexivity | contradiction ].
+      ** unfold alphabet. destruct e ; repeat (try apply in_eq ; try apply in_cons).
+  * rewrite <- (app_nil_l s). constructor; auto.
+- destruct H0 as [c0 [P0 P1]]. rewrite in_map_iff in P0. destruct P0 as [x [P3 P4]]. subst.
+  simpl in P1. destruct (eq_event_dec x e).
+  * inversion P1. inversion H3. subst. simpl. assumption.
+  * inversion P1. inversion H3.
+Qed.
+
+
+Lemma plus_norm_nil : forall (c : Contract), ~([] ==~ plus_fold (map (fun e0 : EventType => Event e0 _;_ plus_norm (c / e0)) alphabet)).
+Proof.
+intros. intro H. apply in_plus_fold in H as [c0 [P0 P1]]. apply in_map_iff in P0 as [e [P P3]]. 
+subst. inversion P1. apply app_eq_nil in H0 as [H0 H00]. subst. inversion H1.
+Qed.
+ 
+Theorem plus_norm_spec : forall (c : Contract)(s : Trace), s ==~ c <-> s ==~ plus_norm c.
+Proof.
+intros. funelim (plus_norm c). destruct (stuck_dec c).
+- apply Stuck_failure. assumption.
+- destruct (nu c) eqn:Heqn.
+  * destruct s.
+    ** split;intros;auto. apply empty_nu. assumption.
+    ** assert (HA: forall (c : Contract), e::s ==~ Success _+_ c <-> e::s ==~ c).
+       { split; intros. inversion H0. inversion H3. assumption. auto. } rewrite HA.
+       apply plus_norm_cons. auto.
+  * destruct s.
+    ** split;intros.
+      *** apply empty_nu in H0. rewrite Heqn in H0. discriminate.
+      *** apply plus_norm_nil in H0 as [].
+    ** apply plus_norm_cons. auto.
+Qed.
+
+
+Inductive Sequential : Contract -> Type :=
+ | SeqFailure : Sequential Failure
+ | SeqSuccess : Sequential Success
+ | SeqEvent e  : Sequential (Event e)
+ | SeqPlus c0 c1 (H0: Sequential c0) (H1 : Sequential c1) : Sequential (c0 _+_ c1)
+ | SeqSeq c0 c1 (H0: Sequential c0) (H1 : Sequential c1) : Sequential (c0 _;_ c1).
+
+Definition bind {A B : Type} (a : option A) (f : A -> option B) : option B :=
+  match a with
+    | Some x => f x
+    | None => None
+  end.
+
+Print option.
+Fixpoint translate_aux (c : Contract) : option CSLC.Contract :=
+match c with
+| Failure => Some CSLC.Failure
+| Success => Some CSLC.Success
+| Event e => Some (CSLC.Event e)
+| c0 _+_ c1 => bind (translate_aux c0) (fun c0' => bind (translate_aux c1) (fun c1' => Some (CSLC.CPlus c0' c1')))
+| c0 _;_ c1 => bind (translate_aux c0) (fun c0' => bind (translate_aux c1) (fun c1' => Some (CSLC.CSeq c0' c1')))
+| c0 _*_ c1 => None
+end.
+
+Lemma translate_aux_sequential : forall (c : Contract), Sequential c -> exists c', translate_aux c = Some c'.
+Proof. 
+intros. induction H.
+- exists CSLC.Failure. reflexivity.
+- exists CSLC.Success. reflexivity.
+- exists (CSLC.Event e). reflexivity.
+- destruct IHSequential1,IHSequential2. exists (CSLC.CPlus x x0).
+  simpl. unfold bind. destruct (translate_aux c0).
+  * destruct (translate_aux c1).
+    ** inversion H1. inversion H2. reflexivity.
+    ** inversion H2.
+  * inversion H1.
+- destruct IHSequential1,IHSequential2. exists (CSLC.CSeq x x0).
+  simpl. unfold bind. destruct (translate_aux c0).
+  * destruct (translate_aux c1).
+    ** inversion H1. inversion H2. reflexivity.
+    ** inversion H2.
+  * inversion H1.
+Qed.
+
+
+
+
+Lemma plus_norm_sequential : forall (c : Contract), Sequential (plus_norm c).
+Proof. 
+intros. funelim (plus_norm c).
+destruct (stuck_dec c).
+- constructor.
+- destruct (nu c).
+  * constructor. constructor. induction alphabet.
+    ** simpl. constructor.
+    ** simpl. repeat constructor. auto. assumption.
+  * induction alphabet.
+    ** simpl. constructor.
+    ** simpl. repeat constructor. auto. assumption.
+Defined.
+
+Definition translate (c : Contract) : option CSLC.Contract := translate_aux (plus_norm c).
+
+
+
+Theorem correct_translation : forall (c : Contract), exists c', translate c = Some c' /\ (forall s, pmatches_comp s c <-> CSLC.matches_comp s c').
+Proof.
+intros. unfold translate. pose proof (translate_aux_sequential (plus_norm_sequential c)).
+destruct H. exists x. split. assumption. split; intros.
+- apply plus_norm_spec in H0. apply translate_aux_spec with (plus_norm c); assumption.
+- apply plus_norm_spec. apply translate_aux_spec with (plus_norm c) x s in H. rewrite H. assumption.
+Qed. 
